Tests/package.lean
@@ -1,2 +1,3 @@
 
 import Tests.DOT.Sanity
+import Tests.DTLC.Sanity
