lakefile.lean
@@ -6,11 +6,13 @@ package «Lp2lc» where
 @[default_target]
 lean_lib «Lp2lc» where
 
+@[default_target] -- compiled but should never publish
+lean_lib «Tests» where
+
 lean_lib «Spike» where
 
 lean_lib «LeanCompiler» where
 
-lean_lib «Tests» where
 
 require aesop from git
   "https://github.com/leanprover-community/aesop" @ "v4.29.0"
